
\(f^{-1} \left( \coprod U_i \right) =_? \coprod_i f^{-1} U_i\)?
%
Yes:
\[
\begin{align}
f^{-1}\left[\bigcup_{i \in I} Y_{i}\right] &=\left\{x \in X \mid f(x) \in \bigcup_{i \in I} Y_{i}\right\} \\
&=\left\{x \in \lambda \mid \quad \exists i \in I \text { such that } f(x) \in Y_{i}\right\} \\
&=\bigcup_{i \in I}\left\{x \in X \mid f(x) \in Y_{i}\right\} \\
&=\bigcup_{i \in I} f^{-1}\left[Y_{i}\right]
\end{align}
\]
%
misc
---

\(f^{-1} \left( \bigcap U_i \right) =_? \bigcap_i f^{-1} U_i\)?
%
Yes
%
misc
---

